Found the value of the exponent

proof/correctness/NTT.py
@@ -1,0 +1,53 @@
+def int2bs (n):
+    return [((n // (2 ** k)) % 2) for k in range (8)]
+    
+def bs2int (l):
+    n = 0
+    for k in range (8):
+        n += l[k] * (2**k)
+    return n
+
+def bitrev (n):
+    return (bs2int(list(reversed(int2bs(n)))))
+
+class exponent:
+
+    def __init__(self):
+        self.f = [[[0 for y in range (2**k)] for x in range (2**k)] for k in range (8)]
+
+    def pp(self, m):
+        for k in range (min(m, 8)):
+            for x in range (2**k):
+                print(self.f[k][x])
+            print()
+
+    def pp_bitrev(self, m):
+        for k in range (min(m, 8)):
+            for x in range (2**k):
+                print(list(map(bitrev, self.f[k][x])))
+            print()
+    
+    def fill_inductive(self):
+        for k in range (7):
+            p = 2**k
+            for x in range (p):
+                for y in range (p):
+                    self.f[k+1][x][y]       = ((self.f[k][x][y]                             ) % 256)
+                    self.f[k+1][x][p+y]     = ((self.f[k][x][y] + (2*x+1) * (2**(6-k))      ) % 256)
+                    self.f[k+1][p+x][y]     = ((self.f[k][x][y]                             ) % 256)
+                    self.f[k+1][p+x][p+y]   = ((self.f[k][x][y] + (2*x+1) * (2**(6-k)) + 128) % 256)
+    
+    def fill_prevision(self):
+        for k in range (8):
+            p = 2**k
+            for x in range (p):
+                for y in range (p):
+                    self.f[k][x][y] = ((2*x + 1) * bitrev(2 * (y % (2**k)))) % 256
+
+e_inductive = exponent()
+e_prevision = exponent()
+e_inductive.fill_inductive()
+e_prevision.fill_prevision()
+#e_inductive.pp(4)
+#e_prevision.pp(4)
+print(e_inductive.f == e_prevision.f)
